feat: EncryptItem and DecryptItem (#22)
* feat: EncryptItem and DecryptItem

* m

* m

* m

* m

* m

* m

* m

* m

* m

DynamoDbItemEncryptor/src/AwsCryptographyDynamoDbItemEncryptorOperations.dfy
@@ -1,13 +1,17 @@
 // Copyright Amazon.com Inc. or its affiliates. All Rights Reserved.
 // SPDX-License-Identifier: Apache-2.0
 include "../Model/AwsCryptographyDynamoDbItemEncryptorTypes.dfy"
-include "StubbedData.dfy"
+include "DynamoToStruct.dfy"
 
 module AwsCryptographyDynamoDbItemEncryptorOperations refines AbstractAwsCryptographyDynamoDbItemEncryptorOperations {
   import ComAmazonawsDynamodbTypes
   import AwsCryptographyMaterialProvidersTypes
   import StructuredEncryption
-  import StubbedData
+  import DynamoToStruct
+  import Base64
+  import opened StandardLibrary
+  import Seq
+  import CSE = AwsCryptographyStructuredEncryptionTypes
 
   datatype Config = Config(
     nameonly tableName: ComAmazonawsDynamodbTypes.TableName,
@@ -25,6 +29,136 @@ module AwsCryptographyDynamoDbItemEncryptorOperations refines AbstractAwsCryptog
 
   type InternalConfig = Config
 
+  // Encode ASCII as UTF8 in a function, to allow use in ensures clause
+  function method {:opaque} {:tailrecursion} EncodeAscii(s : string) : (ret : ValidUTF8Bytes)
+    requires IsASCIIString(s)
+    ensures |s| == |ret|
+    ensures forall i | 0 <= i < |s| :: s[i] as uint8 == ret[i]
+  {
+    if |s| == 0 then
+      []
+    else
+      var x := [s[0] as uint8];
+      assert ValidUTF8Seq(x);
+      ValidUTF8Concat(x, EncodeAscii(s[1..]));
+      x + EncodeAscii(s[1..])
+  }
+
+  // if ascii strings are different, their encoding is also unique
+  lemma EncodeAsciiUnique2(x : string, y : string)
+    requires IsASCIIString(x) && IsASCIIString(y)
+    requires x != y
+    ensures EncodeAscii(x) != EncodeAscii(y)
+  {
+    reveal EncodeAscii();
+    if EncodeAscii(x) == EncodeAscii(y) {
+      if |EncodeAscii(x)| == 0 && |EncodeAscii(y)| == 0 {
+      } else if EncodeAscii(x)[0] == EncodeAscii(y)[0] {
+        assert EncodeAscii(x)[1..] != EncodeAscii(y)[1..] by {
+          EncodeAsciiUnique2(x[1..], y[1..]);
+        }
+      } else {
+      }
+    }
+  }
+
+  // if ascii strings are different, their encoding is also unique
+  lemma {:opaque} EncodeAsciiUnique()
+    ensures forall x : string, y : string :: IsASCIIString(x) && IsASCIIString(y) && x != y ==> EncodeAscii(x) != EncodeAscii(y)
+  {
+    forall x : string, y : string ensures IsASCIIString(x) && IsASCIIString(y) && x != y ==> EncodeAscii(x) != EncodeAscii(y) {
+        if IsASCIIString(x) && IsASCIIString(y) && x != y {
+            EncodeAsciiUnique2(x, y);
+        }
+    }
+  }
+
+  // constant attribute names for the encryption context
+  const TABLE_NAME : seq<uint8> := EncodeAscii("aws-crypto-table-name");
+  const PARTITION_NAME : seq<uint8> := EncodeAscii("aws-crypto-partition-name");
+  const PARTITION_VALUE : seq<uint8> := EncodeAscii("aws-crypto-partition-value");
+  const SORT_NAME : seq<uint8> := EncodeAscii("aws-crypto-sort-name");
+  const SORT_VALUE : seq<uint8> := EncodeAscii("aws-crypto-sort-value");
+
+  // transform AttributeValue into encoded encryption context value
+  function method {:opaque} EncodeValue(val : ComAmazonawsDynamodbTypes.AttributeValue) : Result<ValidUTF8Bytes, string>
+  {
+    var nValue :- DynamoToStruct.TopLevelAttributeToBytes(val);
+    var val64 := Base64.Encode(nValue);
+    Success(EncodeAscii(val64))
+  }
+
+  // create encryption content from DynamoDB item
+  function method {:opaque} MakeEncryptionContextInner(
+    config : InternalConfig,
+    item : ComAmazonawsDynamodbTypes.AttributeMap)
+    : (ret : Result<AwsCryptographyMaterialProvidersTypes.EncryptionContext, string>)
+
+    //= specification/dynamodb-encryption-client/encrypt-item.md#dynamodb-item-base-context
+    //= type=implication
+    //# The DynamoDB Item Base Context MUST contain:
+    //# - the key `TODO:aws-crypto-table-name` with a value equal to the DynamoDB Table Name of the DynamoDB Table
+    //#   this item is stored in (or will be stored in).
+    //# - the key `TODO:aws-crypto-partition-name` with a value equal to the name of the Partition Key on this item.
+    //# - the key `TODO:aws-crypto-partition-value` with a value equal to this item's partition attribute,
+    //#   serialized according to [Attribute Value Serialization](./ddb-attribute-serialization.md#attribute-value-serialization)
+    //#   and [Base 64 encoded](https://www.rfc-editor.org/rfc/rfc4648).
+    //# - If this item has a sort key attribute,
+    //#   the key `TODO:aws-crypto-sort-name` with a value equal to the [DynamoDB Sort Key Name](#dynamodb-sort-key-name).
+    //# - If this item has a sort key attribute,
+    //#   the key `TODO:aws-crypto-sort-value` with a value equal to this item's sort attribute,
+    //#   serialized according to [Attribute Value Serialization](./ddb-attribute-serialization.md#attribute-value-serialization)
+    //#   and [Base 64 encoded](https://www.rfc-editor.org/rfc/rfc4648).
+    ensures ret.Success? ==>
+      && TABLE_NAME in ret.value && UTF8.Encode(config.tableName).Success? && ret.value[TABLE_NAME] == UTF8.Encode(config.tableName).value
+      && PARTITION_NAME in ret.value && UTF8.Encode(config.partitionKeyName).Success? && ret.value[PARTITION_NAME] == UTF8.Encode(config.partitionKeyName).value
+      && config.partitionKeyName in item
+      && PARTITION_VALUE in ret.value && EncodeValue(item[config.partitionKeyName]).Success? && ret.value[PARTITION_VALUE] == EncodeValue(item[config.partitionKeyName]).value
+    ensures ret.Success? && config.sortKeyName.Some? ==>
+      && SORT_NAME in ret.value && UTF8.Encode(config.sortKeyName.value).Success? && ret.value[SORT_NAME] == UTF8.Encode(config.sortKeyName.value).value
+      && config.sortKeyName.value in item
+      && SORT_VALUE in ret.value && EncodeValue(item[config.sortKeyName.value]).Success? && ret.value[SORT_VALUE] == EncodeValue(item[config.sortKeyName.value]).value
+
+    //= specification/dynamodb-encryption-client/encrypt-item.md#dynamodb-item-base-context
+    //= type=implication
+    //# If this item does not have a sort key attribute,
+    //# the DynamoDB Item Context MUST NOT contain the keys
+    //# `TODO:aws-crypto-sort-name` or
+    //# `TODO:aws-crypto-sort-value`.
+    ensures ret.Success? && config.sortKeyName.None? ==>
+      && SORT_NAME !in ret.value
+      && SORT_VALUE !in ret.value
+
+    ensures ret.Success? ==> config.sortKeyName.Some? && config.sortKeyName.value !in item ==> ret.Failure?
+    ensures ret.Success? ==> config.sortKeyName.None? || (config.sortKeyName.value in item)
+    ensures ret.Success? ==> config.partitionKeyName in item
+  {
+    EncodeAsciiUnique();
+    :- Need(config.partitionKeyName in item, "Partition key " + config.partitionKeyName + " not found in Item to be encrypted or decrypted");
+    var tableName :- UTF8.Encode(config.tableName);
+    var partitionName :- UTF8.Encode(config.partitionKeyName);
+    var partitionValue :- EncodeValue(item[config.partitionKeyName]);
+    var retval := map[TABLE_NAME := tableName, PARTITION_NAME := partitionName, PARTITION_VALUE := partitionValue];
+    if config.sortKeyName.None? then
+      Success(retval)
+    else
+      :- Need(config.sortKeyName.value in item, "Sort key " + config.sortKeyName.value + " not found in Item to be encrypted or decrypted");
+      var sortName :- UTF8.Encode(config.sortKeyName.value);
+      var sortValue :- EncodeValue(item[config.sortKeyName.value]);
+      Success(retval + map[SORT_NAME := sortName, SORT_VALUE := sortValue])
+  }
+
+  // translate to Error type
+  function method MakeEncryptionContext(
+    config : InternalConfig,
+    item : ComAmazonawsDynamodbTypes.AttributeMap)
+    : (ret : Result<AwsCryptographyMaterialProvidersTypes.EncryptionContext, Error>)
+    ensures ret.Success? ==> config.sortKeyName.Some? && config.sortKeyName.value !in item ==> ret.Failure?
+    ensures ret.Success? ==> config.sortKeyName.None? || config.sortKeyName.value in item
+  {
+    DynamoToStruct.MapError(MakeEncryptionContextInner(config, item))
+  }
+
   predicate ValidInternalConfig?(config: InternalConfig)
   {
     && config.cmm.ValidState()
@@ -38,111 +172,372 @@ module AwsCryptographyDynamoDbItemEncryptorOperations refines AbstractAwsCryptog
     + config.structuredEncryption.Modifies
   }
 
+  // return proper Crypto Action by name
+  function method GetCryptoSchemaActionInner(
+    config : InternalConfig,
+    attr : ComAmazonawsDynamodbTypes.AttributeName)
+    : (ret : Result<CSE.CryptoAction, string>)
+    ensures (attr !in config.attributeActions && !DoNotSign(config, attr)) ==> ret.Failure?
+  {
+    :- CheckConsistantSpec(config, attr);
+    if attr in config.attributeActions then
+      Success(config.attributeActions[attr])
+    else if DoNotSign(config, attr) then
+      Success(CSE.CryptoAction.DO_NOTHING)
+    else
+      Failure("No Crypto Action configured for attribute " + attr)
+  }
+
+  // get Crypto Action and wrap in CryptoSchema
+  function method GetCryptoSchemaAction(
+    config : InternalConfig,
+    attr : ComAmazonawsDynamodbTypes.AttributeName)
+    : (ret : Result<CSE.CryptoSchema, string>)
+    ensures (attr !in config.attributeActions && !DoNotSign(config, attr)) ==> ret.Failure?
+  {
+    var action :- GetCryptoSchemaActionInner(config, attr);
+    var newElement := CSE.CryptoSchemaContent.Action(action);
+    Success(CSE.CryptoSchema(content := newElement, attributes := None))
+  }
+
+  // The same attr must not be in two places
+  predicate method InvalidSpec(config : InternalConfig, attr : ComAmazonawsDynamodbTypes.AttributeName)
+  {
+    attr in config.attributeActions && 
+      (|| (config.allowedUnauthenticatedAttributes.Some? && attr in config.allowedUnauthenticatedAttributes.value)
+      || (config.allowedUnauthenticatedAttributePrefix.Some? && config.allowedUnauthenticatedAttributePrefix.value <= attr))
+  }
+
+  function method CheckConsistantSpec(config : InternalConfig, attr : ComAmazonawsDynamodbTypes.AttributeName) : Outcome<string> {
+    if InvalidSpec(config, attr) then
+      Fail("Attribute " + attr + " is configures both as an explicit attribute and as an implicit unauthenticated attribute.")
+    else
+      Pass
+  }
+
+  // Attr must not be part of signature
+  predicate method DoNotSign(config : InternalConfig, attr : ComAmazonawsDynamodbTypes.AttributeName)
+  {
+    || (attr in config.attributeActions && config.attributeActions[attr] == CSE.CryptoAction.DO_NOTHING)
+    || (config.allowedUnauthenticatedAttributes.Some? && attr in config.allowedUnauthenticatedAttributes.value)
+    || (config.allowedUnauthenticatedAttributePrefix.Some? && config.allowedUnauthenticatedAttributePrefix.value <= attr)
+  }
+
+  // Attr must be part of signature
+  predicate method InSignatureScope(config : InternalConfig, attr : ComAmazonawsDynamodbTypes.AttributeName) {
+    !DoNotSign(config, attr)
+  }
+
+  // return proper Authenticate Action by name
+  function method GetAuthenticateSchemaActionInner(
+    config : InternalConfig,
+    attr : ComAmazonawsDynamodbTypes.AttributeName)
+    : (ret : Result<CSE.AuthenticateAction, string>)
+
+    //= specification/dynamodb-encryption-client/decrypt-item.md#signature-scope
+    //= type=implication
+    //# An Attribute on a DynamoDB Item MUST NOT be considered as within the signature scope
+    //# if it's Attribute Name is included in [Unauthenticated Attributes](./ddb-item-encryptor.md#unauthenticated-attributes)
+    //# or if it's Attribute Name begins with the prefix specified in
+    //# [Unauthenticated Attribute Prefix](./ddb-item-encryptor.md#unauthenticated-attribute-prefix).
+
+    //= specification/dynamodb-encryption-client/decrypt-item.md#signature-scope
+    //= type=implication
+    //# Otherwise, Attributes MUST be considered as within the signature scope.
+    ensures ret.Success? ==>
+      ret.value == CSE.AuthenticateAction.DO_NOT_SIGN <==> DoNotSign(config, attr)
+
+    //= specification/dynamodb-encryption-client/decrypt-item.md#signature-scope
+    //= type=implication
+    //# If an Authenticate Action other than DO_NOTHING is configured for an attribute name included in [Unauthenticated Attributes](./ddb-item-encryptor.md#unauthenticated-attributes)
+    //# or beginning with the prefix specified in [Unauthenticated Attribute Prefix](./ddb-item-encryptor.md#unauthenticated-attribute-prefix),
+    //# this operation MUST yield an error.
+    ensures
+      && attr in config.attributeActions
+      && config.attributeActions[attr] != CSE.CryptoAction.DO_NOTHING
+      && DoNotSign(config, attr)
+      ==> ret.Failure?
+  {
+    :- CheckConsistantSpec(config, attr);
+    if DoNotSign(config, attr) then
+      Success(CSE.AuthenticateAction.DO_NOT_SIGN)
+    else
+      Success(CSE.AuthenticateAction.SIGN)
+  }
+
+  // get Authenticate Action and wrap in AuthenticateSchema
+  function method GetAuthenticateSchemaAction(
+    config : InternalConfig,
+    attr : ComAmazonawsDynamodbTypes.AttributeName)
+    : Result<CSE.AuthenticateSchema, string>
+  {
+    var newElement :- GetAuthenticateSchemaActionInner(config, attr);
+    var newElement := CSE.AuthenticateSchemaContent.Action(newElement);
+    Success(CSE.AuthenticateSchema(content := newElement, attributes := None))
+  }
+
+  // get CryptoSchema for this item
+  function method ConfigToCryptoSchema(
+    config : InternalConfig,
+    item : ComAmazonawsDynamodbTypes.AttributeMap)
+    : (ret : Result<CSE.CryptoSchema, Error>)
+
+    //= specification/dynamodb-encryption-client/encrypt-item.md#behavior
+    //= type=implication
+    //# The [Attributes Actions](./ddb-item-encryptor.md#attribute-actions)
+    //# configured on this Item Encryptor MUST specify a Crypto Action
+    //# for every attribute in the [input DynamoDB Item](#dynamodb-item)
+    //# (Attribute Actions MAY specify a Crypto Action for an attribute not
+    //# in the input DynamoDB Item).
+    ensures forall k <- item.Keys ::
+      (k !in config.attributeActions && !DoNotSign(config, k)) ==> ret.Failure?
+
+    //= specification/dynamodb-encryption-client/encrypt-item.md#behavior
+    //= type=implication
+    //# - The Crypto Schema MUST NOT contain more Crypto Actions than those specified by the previous point.
+    ensures ret.Success? ==> ret.value.content.SchemaMap? && item.Keys == ret.value.content.CryptoSchemaMap.Keys
+
+    //= specification/dynamodb-encryption-client/encrypt-item.md#behavior
+    //= type=implication
+    //# - For every attribute on the input Item,
+    //# there MUST exist a Crypto Action in the Crypto Schema
+    //# such that the Crypto Action indexed by that attribute name in the Crypto Schema
+    //# equals the Crypto Action indexed by that attribute name in the configured Attribute Actions.
+    ensures ret.Success? ==> forall k <-item.Keys ::
+      && GetCryptoSchemaAction(config, k).Success?
+      && ret.value.content.CryptoSchemaMap[k] == GetCryptoSchemaAction(config, k).value
+      && (k in config.attributeActions ==>
+        ret.value.content.CryptoSchemaMap[k].content ==
+        CSE.CryptoSchemaContent.Action(config.attributeActions[k]))
+  {
+    var schema := map kv <- item.Items | true :: kv.0 := GetCryptoSchemaAction(config, kv.0);
+    DynamoToStruct.MapKeysMatchItems(item);
+    DynamoToStruct.SimplifyMapValueSuccess(schema);
+    var actionMapRes := DynamoToStruct.SimplifyMapValue(schema);
+    assert actionMapRes.Failure? ==> exists kv <- item.Items :: GetCryptoSchemaAction(config, kv.0).Failure?;
+    assert actionMapRes.Failure? <==> exists k <- item.Keys :: schema[k].Failure?;
+    assert actionMapRes.Failure? <==> exists k <- item.Keys :: GetCryptoSchemaAction(config, k).Failure?;
+
+    var actionMap :- DynamoToStruct.MapError(actionMapRes);
+    var schemaContent := CSE.CryptoSchemaContent.SchemaMap(actionMap);
+    var finalSchema := CSE.CryptoSchema(content := schemaContent, attributes := None);
+    Success(finalSchema)
+  }
+
+  // get AuthenticateSchema for this item
+  function method ConfigToAuthenticateSchema(
+    config : InternalConfig,
+    item : ComAmazonawsDynamodbTypes.AttributeMap)
+    : (ret : Result<CSE.AuthenticateSchema, Error>)
+
+    //= specification/dynamodb-encryption-client/decrypt-item.md#behavior
+    //= type=implication
+    //# - The number of Authenticate Actions in the Authenticate Schema
+    //# MUST EQUAL the number of Attributes on the [input DynamoDB Item](#dynamodb-item).
+    ensures ret.Success? ==> ret.value.content.SchemaMap? && item.Keys == ret.value.content.AuthenticateSchemaMap.Keys
+
+    //= specification/dynamodb-encryption-client/decrypt-item.md#behavior
+    //= type=implication
+    //# - For every Attribute in the [input DynamoDB Item](#dynamodb-item)
+    //# that is not in the [signature scope](#signature-scope),
+    //# there MUST exist a [DO_NOT_SIGN Authenticate Action](../structured-encryption/structures.md#do_not_sign)
+    //# in the Authenticate Schema,
+    //# string indexed at the top level by that attribute name.
+    ensures ret.Success? ==> forall k <-item.Keys ::
+      !InSignatureScope(config, k) ==>
+      ret.value.content.AuthenticateSchemaMap[k].content ==
+      CSE.AuthenticateSchemaContent.Action(CSE.AuthenticateAction.DO_NOT_SIGN)
+
+    //= specification/dynamodb-encryption-client/decrypt-item.md#behavior
+    //= type=implication
+    //# - For every Attribute in the [input DynamoDB Item](#dynamodb-item)
+    //# that is in the [signature scope](#signature-scope),
+    //# there MUST exist a [SIGN Authenticate Action](../structured-encryption/structures.md#sign)
+    //# in the Authenticate Schema,
+    //# string indexed at the top level by that attribute name.
+    ensures ret.Success? ==> forall k <-item.Keys ::
+      && GetAuthenticateSchemaAction(config, k).Success?
+      && InSignatureScope(config, k) ==>
+        ret.value.content.AuthenticateSchemaMap[k].content ==
+        CSE.AuthenticateSchemaContent.Action(CSE.AuthenticateAction.SIGN)
+  {
+    var schema := map kv <- item.Items | true :: kv.0 := GetAuthenticateSchemaAction(config, kv.0);
+    DynamoToStruct.MapKeysMatchItems(item);
+    var authMap :- DynamoToStruct.MapError(DynamoToStruct.SimplifyMapValue(schema));
+    var schemaContent := CSE.AuthenticateSchemaContent.SchemaMap(authMap);
+    var finalSchema := CSE.AuthenticateSchema(content := schemaContent, attributes := None);
+    Success(finalSchema)
+  }
+
   predicate EncryptItemEnsuresPublicly(input: EncryptItemInput, output: Result<EncryptItemOutput, Error>)
   {true}
 
+  // public Encrypt method
   method EncryptItem(config: InternalConfig, input: EncryptItemInput)
-      returns (output: Result<EncryptItemOutput, Error>)
-  {
-    // TODO transform our input DDB item into a Structure the SEL can understand.
-    // TODO transform attributeActions into a CryptoSchema that the SEL can understand
-    // For now, just pass some stubbed input
-    var plaintextStructure := StubbedData.STUBBED_STRUCTURED_DATA;
-    var cryptoSchema := StubbedData.STUBBED_CRYPTO_SCHEMA;
+    returns (output: Result<EncryptItemOutput, Error>)
+    //= specification/dynamodb-encryption-client/encrypt-item.md#dynamodb-item
+    //= type=implication
+    //# This item MUST include an Attribute with a name that matches the
+    //# [DynamoDB Partition Key Name](./ddb-item-encryptor.md#dynamodb-partition-key-name)
+    //# configured on the [DynamoDB Item Encryptor](./ddb-item-encryptor.md).
+    ensures output.Success? ==> config.partitionKeyName in input.plaintextItem
 
-    // Use the structured encryption client to decrypt the item.
+    //= specification/dynamodb-encryption-client/encrypt-item.md#dynamodb-item
+    //= type=implication
+    //# Otherwise this operation MUST yield an error.
+    ensures config.partitionKeyName !in input.plaintextItem ==> output.Failure?
+
+    //= specification/dynamodb-encryption-client/encrypt-item.md#dynamodb-item
+    //= type=implication
+    //# If the [DynamoDB Item Encryptor](./ddb-item-encryptor.md)
+    //# has a [DynamoDB Sort Key Name](./ddb-item-encryptor.md#dynamodb-sort-key-name) configured,
+    //# this item MUST include an Attribute with that name.
+    ensures output.Success? ==> (config.sortKeyName.None? || config.sortKeyName.value in input.plaintextItem)
+
+    // Otherwise this operation MUST yield an error.
+    ensures config.sortKeyName.Some? && config.sortKeyName.value !in input.plaintextItem ==> output.Failure?
+
+    ensures output.Success? ==>
+      //= specification/dynamodb-encryption-client/encrypt-item.md#behavior
+      //= type=implication
+      //# Given the converted [Structured Data](../structured-encryption/structures.md#structured-data),
+      //# this operation MUST delegate encryption of this data to
+      //# Structured Encryption Client's [Encrypt Structure](../structured-encryption/encrypt-structure.md),
+      //# with the following inputs:
+      && (|config.structuredEncryption.History.EncryptStructure| == |old(config.structuredEncryption.History.EncryptStructure)| + 1)
+      && (Seq.Last(config.structuredEncryption.History.EncryptStructure).output.Success?)
+
+      //= specification/dynamodb-encryption-client/encrypt-item.md#behavior
+      //= type=implication
+      //# - Crypto Schema MUST be a [Crypto Schema](../structured-encryption/structures.md#crypto-schema)
+      //# analogous to the [configured Attribute Actions](./ddb-item-encryptor.md#attribute-actions).
+      && ConfigToCryptoSchema(config, input.plaintextItem).Success?
+      && Seq.Last(config.structuredEncryption.History.EncryptStructure).input.cryptoSchema
+        == ConfigToCryptoSchema(config, input.plaintextItem).value
+
+      //= specification/dynamodb-encryption-client/encrypt-item.md#behavior
+      //= type=implication
+      //# - Structured Data MUST be the Structured Data converted above.
+      && DynamoToStruct.ItemToStructured(input.plaintextItem).Success?
+      && Seq.Last(config.structuredEncryption.History.EncryptStructure).input.plaintextStructure
+        == CSE.StructuredData(
+          content := CSE.StructuredDataContent.DataMap(DynamoToStruct.ItemToStructured(input.plaintextItem).value),
+          attributes := None)
+
+      //= specification/dynamodb-encryption-client/encrypt-item.md#behavior
+      //= type=implication
+      //# - Encryption Context MUST be this input Item's [DynamoDB Item Base Context](#dynamodb-item-base-context).
+      && MakeEncryptionContext(config, input.plaintextItem).Success?
+      && Seq.Last(config.structuredEncryption.History.EncryptStructure).input.encryptionContext
+        == Some(MakeEncryptionContext(config, input.plaintextItem).value)
+  {
+    var context :- MakeEncryptionContext(config, input.plaintextItem);
+    var plaintextStructure :- DynamoToStruct.ItemToStructured(input.plaintextItem);
+    var cryptoSchema :- ConfigToCryptoSchema(config, input.plaintextItem);
+    var wrappedStruct := CSE.StructuredData(
+      content := CSE.StructuredDataContent.DataMap(plaintextStructure),
+      attributes := None);
+
     var encryptRes := config.structuredEncryption.EncryptStructure(
-      AwsCryptographyStructuredEncryptionTypes.EncryptStructureInput(
-        plaintextStructure:=plaintextStructure,
+      CSE.EncryptStructureInput(
+        plaintextStructure:=wrappedStruct,
         cryptoSchema:=cryptoSchema,
         cmm:=config.cmm,
-        encryptionContext:=None()
+        encryptionContext:=Some(context)
       )
     );
-    // TODO properly convert error and bubble up message
-    :- Need(encryptRes.Success?,
-      Error.DynamoDbItemEncryptorException(
-        message := "Failed to encrypt item."));
-    var encryptedData := encryptRes.value.encryptedStructure;
-
-    // TODO convert the encrypted structure back into a DDB item.
-    // For now we use knowledge of the expected output 
-    // (StructuredEncryption.DecryptStructure is just a passthrough)
-    // to quickly construct a related DDB item.
-    expect encryptedData.content.DataMap?;
-    expect "foo" in encryptedData.content.StructuredDataMap;
-    expect "bar" in encryptedData.content.StructuredDataMap;
-    expect "fizzbuzz" in encryptedData.content.StructuredDataMap;
-    expect encryptedData.content.StructuredDataMap["foo"].content.Terminal?;
-    expect encryptedData.content.StructuredDataMap["bar"].content.Terminal?;
-    expect encryptedData.content.StructuredDataMap["fizzbuzz"].content.Terminal?;
-    var stubbedItem := map[
-      "foo" := ComAmazonawsDynamodbTypes.AttributeValue.B(
-        BinaryAttributeValue:=encryptedData.content.StructuredDataMap["foo"].content.StructuredDataTerminal.value
-      ),
-      "bar" := ComAmazonawsDynamodbTypes.AttributeValue.B(
-        BinaryAttributeValue:=encryptedData.content.StructuredDataMap["bar"].content.StructuredDataTerminal.value
-      ),
-      "fizzbuzz" := ComAmazonawsDynamodbTypes.AttributeValue.B(
-        BinaryAttributeValue:=encryptedData.content.StructuredDataMap["fizzbuzz"].content.StructuredDataTerminal.value
-      )
-    ];
-
-    var encryptOutput := EncryptItemOutput(encryptedItem := stubbedItem);
-    output := Success(encryptOutput);
+    var encryptVal :- encryptRes.MapFailure(e => Error.AwsCryptographyStructuredEncryption(e));
+    var encryptedData := encryptVal.encryptedStructure;
+    var ddbItem :- DynamoToStruct.StructuredToItem(encryptedData.content.StructuredDataMap);
+    output := Success(EncryptItemOutput(encryptedItem := ddbItem));
   }
 
   predicate DecryptItemEnsuresPublicly(input: DecryptItemInput, output: Result<DecryptItemOutput, Error>)
   {true}
-  
-  method DecryptItem(config: InternalConfig, input: DecryptItemInput)
-      returns (output: Result<DecryptItemOutput, Error>)
-  {
-    // TODO transform our input DDB item into a Structure the SEL can understand.
-    // TODO calculate AuthenticateSchema based on input DDB Item and AllowedAuthenticated* fields
-    // For now, just pass some stubbed input
-    var encryptedStructure := StubbedData.STUBBED_STRUCTURED_DATA;
-    var authenticateSchema := StubbedData.STUBBED_AUTHENTICATE_SCHEMA;
 
-    // Use the structured encryption client to decrypt the item.
+  // public Decrypt method
+  method DecryptItem(config: InternalConfig, input: DecryptItemInput)
+    returns (output: Result<DecryptItemOutput, Error>)
+
+    //= specification/dynamodb-encryption-client/decrypt-item.md#dynamodb-item
+    //= type=implication
+    //# This item MUST include an Attribute with a name that matches the
+    //# [DynamoDB Partition Key Name](./ddb-item-encryptor.md#dynamodb-partition-key-name)
+    //# configured on the [DynamoDB Item Encryptor](./ddb-item-encryptor.md).
+    ensures output.Success? ==> config.partitionKeyName in input.encryptedItem
+
+    //= specification/dynamodb-encryption-client/decrypt-item.md#dynamodb-item
+    //= type=implication
+    //# Otherwise this operation MUST yield an error.
+    ensures config.partitionKeyName !in input.encryptedItem ==> output.Failure?
+
+    //= specification/dynamodb-encryption-client/decrypt-item.md#dynamodb-item
+    //= type=implication
+    //# If the [DynamoDB Item Encryptor](./ddb-item-encryptor.md)
+    //# has a [DynamoDB Sort Key Name](./ddb-item-encryptor.md#dynamodb-sort-key-name) configured,
+    //# this item MUST include an Attribute with that name.
+    ensures output.Success? ==> config.sortKeyName.None? || config.sortKeyName.value in input.encryptedItem
+
+    // Otherwise this operation MUST yield an error.
+    ensures config.sortKeyName.Some? && config.sortKeyName.value !in input.encryptedItem ==> output.Failure?
+
+    ensures output.Success? ==>
+      //= specification/dynamodb-encryption-client/decrypt-item.md#behavior
+      //= type=implication
+      //# Given the converted [Structured Data](../structured-encryption/structures.md#structured-data),
+      //# this operation MUST delegate decryption of this data to
+      //# Structured Encryption Client's [Decrypt Structure](../structured-encryption/encrypt-structure.md),
+      //# with the following inputs:
+      && (|config.structuredEncryption.History.DecryptStructure| == |old(config.structuredEncryption.History.DecryptStructure)| + 1)
+      && (Seq.Last(config.structuredEncryption.History.DecryptStructure).output.Success?)
+
+      //= specification/dynamodb-encryption-client/decrypt-item.md#behavior
+      //= type=implication
+      //# - Authenticate Schema MUST be a [Authenticate Schema](../structured-encryption/structures.md#crypto-schema)
+      //# built with the following requirements:
+      && ConfigToAuthenticateSchema(config, input.encryptedItem).Success?
+      && Seq.Last(config.structuredEncryption.History.DecryptStructure).input.authenticateSchema
+        == ConfigToAuthenticateSchema(config, input.encryptedItem).value
+
+      //= specification/dynamodb-encryption-client/decrypt-item.md#behavior
+      //= type=implication
+      //# - CMM MUST be the [CMM configured on this Item Encryptor](./ddb-item-encryptor.md#cmm).
+      && Seq.Last(config.structuredEncryption.History.DecryptStructure).input.cmm == config.cmm
+
+      //= specification/dynamodb-encryption-client/decrypt-item.md#behavior
+      //= type=implication
+      //# - Encryption Context MUST be the input Item's [DynamoDB Item Base Context](./encrypt-item.md#dynamodb-item-base-context).
+      && MakeEncryptionContext(config, input.encryptedItem).Success?
+      && Seq.Last(config.structuredEncryption.History.DecryptStructure).input.encryptionContext
+        == Some(MakeEncryptionContext(config, input.encryptedItem).value)
+
+      //= specification/dynamodb-encryption-client/decrypt-item.md#behavior
+      //= type=implication
+      //# - Encrypted Structured Data MUST be the Structured Data converted above.
+      && DynamoToStruct.ItemToStructured(input.encryptedItem).Success?
+      && Seq.Last(config.structuredEncryption.History.DecryptStructure).input.encryptedStructure
+        == CSE.StructuredData(
+          content := CSE.StructuredDataContent.DataMap(DynamoToStruct.ItemToStructured(input.encryptedItem).value),
+          attributes := None)
+  {
+    var context :- MakeEncryptionContext(config, input.encryptedItem);
+    var encryptedStructure :- DynamoToStruct.ItemToStructured(input.encryptedItem);
+    var authenticateSchema :- ConfigToAuthenticateSchema(config, input.encryptedItem);
+    var wrappedStruct := CSE.StructuredData(
+      content := CSE.StructuredDataContent.DataMap(encryptedStructure),
+      attributes := None);
+
     var decryptRes := config.structuredEncryption.DecryptStructure(
-      AwsCryptographyStructuredEncryptionTypes.DecryptStructureInput(
-        encryptedStructure:=encryptedStructure,
+      CSE.DecryptStructureInput(
+        encryptedStructure:=wrappedStruct,
         authenticateSchema:=authenticateSchema,
         cmm:=config.cmm,
-        encryptionContext:=None()
+        encryptionContext:=Some(context)
       )
     );
-    // TODO properly convert error and bubble up message
-    :- Need(decryptRes.Success?,
-      Error.DynamoDbItemEncryptorException(
-        message := "Failed to decrypt item."));
-    var decryptedData := decryptRes.value.plaintextStructure;
-
-    // TODO convert the encrypted structure back into a DDB item.
-    // For now we use knowledge of the expected output 
-    // (StructuredEncryption.EncryptStructure is just a passthrough)
-    // to quickly construct a related DDB item.
-    expect decryptedData.content.DataMap?;
-    expect "foo" in decryptedData.content.StructuredDataMap;
-    expect "bar" in decryptedData.content.StructuredDataMap;
-    expect "fizzbuzz" in decryptedData.content.StructuredDataMap;
-    expect decryptedData.content.StructuredDataMap["foo"].content.Terminal?;
-    expect decryptedData.content.StructuredDataMap["bar"].content.Terminal?;
-    expect decryptedData.content.StructuredDataMap["fizzbuzz"].content.Terminal?;
-    var stubbedItem := map[
-      "foo" := ComAmazonawsDynamodbTypes.AttributeValue.B(
-        BinaryAttributeValue:=decryptedData.content.StructuredDataMap["foo"].content.StructuredDataTerminal.value
-      ),
-      "bar" := ComAmazonawsDynamodbTypes.AttributeValue.B(
-        BinaryAttributeValue:=decryptedData.content.StructuredDataMap["bar"].content.StructuredDataTerminal.value
-      ),
-      "fizzbuzz" := ComAmazonawsDynamodbTypes.AttributeValue.B(
-        BinaryAttributeValue:=decryptedData.content.StructuredDataMap["fizzbuzz"].content.StructuredDataTerminal.value
-      )
-    ];
-
-    var decryptOutput := DecryptItemOutput(plaintextItem := stubbedItem);
-    output := Success(decryptOutput);
+    var decryptVal :- decryptRes.MapFailure(e => Error.AwsCryptographyStructuredEncryption(e));
+    var decryptedData := decryptVal.plaintextStructure;
+    var ddbItem :- DynamoToStruct.StructuredToItem(decryptedData.content.StructuredDataMap);
+    output := Success(DecryptItemOutput(plaintextItem := ddbItem));
   }
 }
