StructuredEncryption/src/AwsCryptographyStructuredEncryptionOperations.dfy
@@ -16,8 +16,12 @@ module AwsCryptographyStructuredEncryptionOperations refines AbstractAwsCryptogr
 
   predicate EncryptStructureEnsuresPublicly(
     input: EncryptStructureInput, 
-    output: Result<EncryptStructureOutput, Error>)
-  {true}
+    output: Result<EncryptStructureOutput, Error>) {
+      // Input and output types must be the same, and this constraint is useful to Dafny users
+    && (output.Success? && input.plaintextStructure.content.DataMap? ==> output.value.encryptedStructure.content.DataMap?)
+    && (output.Success? && input.plaintextStructure.content.DataList? ==> output.value.encryptedStructure.content.DataList?)
+    && (output.Success? && input.plaintextStructure.content.Terminal? ==> output.value.encryptedStructure.content.Terminal?)
+  }
 
   method EncryptStructure(config: InternalConfig, input: EncryptStructureInput)
       returns (output: Result<EncryptStructureOutput, Error>)
@@ -29,8 +33,12 @@ module AwsCryptographyStructuredEncryptionOperations refines AbstractAwsCryptogr
 
   predicate DecryptStructureEnsuresPublicly(
     input: DecryptStructureInput, 
-    output: Result<DecryptStructureOutput, Error>)
-  {true}
+    output: Result<DecryptStructureOutput, Error>) {
+      // Input and output types must be the same, and this constraint is useful to Dafny users
+    && (output.Success? && input.encryptedStructure.content.DataMap? ==> output.value.plaintextStructure.content.DataMap?)
+    && (output.Success? && input.encryptedStructure.content.DataList? ==> output.value.plaintextStructure.content.DataList?)
+    && (output.Success? && input.encryptedStructure.content.Terminal? ==> output.value.plaintextStructure.content.Terminal?)
+}
   
   method DecryptStructure(config: InternalConfig, input: DecryptStructureInput)
       returns (output: Result<DecryptStructureOutput, Error>)
